tools/ImportFStarTypes/src/main.fs
@@ -9,6 +9,10 @@ exception InternalErr of string
 exception LocErr of loc * exn
 let err (s:string):'a = raise (Err s)
 
+// REVIEW: the type checker doesn't (yet) care what's in the requires/ensures clauses for imported declarations;
+// is there any reason to keep them?
+let keep_req_ens = false;
+
 type string_tree_raw =
 | StLeaf of string
 | StList of string * string * string_tree list
@@ -26,6 +30,7 @@ let st_paren = make_st_list "(" ")"
 let st_angle = make_st_list "<" ">"
 let st_brace = make_st_list "{" "}"
 let st_bracket = make_st_list "[" "]"
+let st_hash_bracket = make_st_list "#[" "]"
 
 let list_opt (m:'a option) (f:'a -> 'b list):'b list = match m with None -> [] | Some x -> f x in
 
@@ -125,7 +130,7 @@ let rec tree_of_univ (u:univ):string_tree =
   | UPlus (u1, u2) -> st_paren [tree_of_univ u1; st_leaf " + "; tree_of_univ u2]
   | UMax us -> st_paren (st_leaf "max" :: List.map tree_of_univ us)
 
-let rec tree_of_exp (e:exp):string_tree =
+let rec tree_of_exp (e:f_exp):string_tree =
   let r = tree_of_exp in
   match e with
   | EId x -> tree_of_id x
@@ -151,31 +156,31 @@ let rec tree_of_exp (e:exp):string_tree =
   | ELet (b, e1, e2) -> st_paren [st_leaf "let"; tree_of_binder b; st_leaf "="; r e1; st_leaf "in"; r e2]
   | EFun (bs, e) -> st_paren ([st_leaf "fun"] @ trees_of_binders bs @ [st_leaf "->"; r e])
   | EUnsupported s -> st_paren [st_leaf "UNSUPPORTED"; st_leaf ("\"" + s + "\"")]
-and tree_of_aqual_exp ((a:aqual), (e:exp)):string_tree =
+and tree_of_aqual_exp ((a:aqual), (e:f_exp)):string_tree =
   tree_of_aqual a (tree_of_exp e)
-and tree_of_binder ((a, x, tOpt):binder):string_tree =
+and tree_of_binder ((a, x, tOpt):f_binder):string_tree =
   let st =
     match tOpt with
     | None -> tree_of_id x
     | Some t -> st_list [st_list [tree_of_id x; st_leaf ":"]; tree_of_exp t]
   in
   tree_of_aqual a st
-and trees_of_binders (bs:binder list):string_tree list =
+and trees_of_binders (bs:f_binder list):string_tree list =
   List.map tree_of_binder bs
 
-let string_of_exp (e:exp):string =
+let string_of_exp (e:f_exp):string =
   string_of_tree (tree_of_exp e)
 
-let tree_of_decl (d:decl):string_tree =
+let tree_of_decl (d:f_decl):string_tree =
   let
     {
-      d_name = x;
-      d_qualifiers = quals;
-      d_category = category;
-      d_udecls = udecls;
-      d_binders = bs;
-      d_typ = t;
-      d_body = body_opt;
+      f_name = x;
+      f_qualifiers = quals;
+      f_category = category;
+      f_udecls = udecls;
+      f_binders = bs;
+      f_typ = t;
+      f_body = body_opt;
     }
     = d
     in
@@ -218,7 +223,7 @@ let get_aqual (e:raw_exp):aqual * raw_exp =
   | RList [(RHash _ | RHashDot _); e] -> (Implicit, e)
   | _ -> (Explicit, e)
 
-let rec parse_exp (e:raw_exp):exp =
+let rec parse_exp (e:raw_exp):f_exp =
   match e with
   | RId (_, x) -> EId (parse_id x)
   | RInt (_, i) -> EInt i
@@ -253,7 +258,7 @@ let rec parse_exp (e:raw_exp):exp =
   | RList [RRefine _; RList [RColon _; RId (_, x); e1]; e2] -> ERefine (parse_id x, parse_exp e1, parse_exp e2)
   | RList [RAscribed _; e1; e2] -> ETyped (parse_exp e1, parse_exp e2)
   | RList [RPattern _; RList pats; e] ->
-      let f (e:raw_exp):exp list =
+      let f (e:raw_exp):f_exp list =
         match e with
         | RList es -> List.map parse_exp es
         | _ -> err ("parse_exp: EPattern: " + string_of_raw_exp e)
@@ -263,16 +268,16 @@ let rec parse_exp (e:raw_exp):exp =
   | RList [RFun _; RList bs; e] -> EFun (List.map parse_binder bs, parse_exp e)
 //  | RList (e::_) | e -> EUnsupported (string_of_raw_exp e)
   | e -> EUnsupported (string_of_raw_exp e)
-and parse_aqual_exp (e:raw_exp):(aqual * exp) =
+and parse_aqual_exp (e:raw_exp):(aqual * f_exp) =
   let (a, e) = get_aqual e in
   (a, parse_exp e)
-and parse_comma_exps (es:raw_exp list):exp list =
+and parse_comma_exps (es:raw_exp list):f_exp list =
   match es with
   | [] -> []
   | (RComma _)::es -> parse_comma_exps es
   | e::es -> (parse_exp e)::(parse_comma_exps es)
-and parse_binder (e:raw_exp):binder = parse_binder_a Explicit e
-and parse_binder_a (a:aqual) (e:raw_exp):binder =
+and parse_binder (e:raw_exp):f_binder = parse_binder_a Explicit e
+and parse_binder_a (a:aqual) (e:raw_exp):f_binder =
   match e with
   | RId (_, x) -> (a, parse_id x, None)
   | RList [RColon _; RId (_, x); t] -> (a, parse_id x, Some (parse_exp t))
@@ -285,35 +290,35 @@ let parse_qualifier (e:raw_exp):string =
   | RQualifier (_, s) -> s
   | _ -> err ("parse_qualifier: " + string_of_raw_exp e)
 
-let parse_decl (e:raw_exp):decl =
+let parse_decl (e:raw_exp):f_decl =
   match e with
   | RList [RList quals; RDecl (_, category); RId (_, x); RList udecls; RList bs; t; body_opt] ->
       {
-        d_name = x;
-        d_qualifiers = List.map parse_qualifier quals
-        d_category = category;
-        d_udecls = List.map parse_rid udecls;
-        d_binders = List.map parse_binder bs;
-        d_typ = parse_exp t;
-        d_body = match body_opt with RList [] -> None | RList [e] -> Some (parse_exp e) | _ -> err ("body: " + string_of_raw_exp body_opt);
+        f_name = x;
+        f_qualifiers = List.map parse_qualifier quals
+        f_category = category;
+        f_udecls = List.map parse_rid udecls;
+        f_binders = List.map parse_binder bs;
+        f_typ = parse_exp t;
+        f_body = match body_opt with RList [] -> None | RList [e] -> Some (parse_exp e) | _ -> err ("body: " + string_of_raw_exp body_opt);
       }
   | _ -> err ("parse_decl: " + string_of_raw_exp e)
 
-let filter_decls (ds:decl list):decl list =
-  let filter_decl_pair ((d:decl option), (dnext:decl option)):decl list =
+let filter_decls (ds:f_decl list):f_decl list =
+  let filter_decl_pair ((d:f_decl option), (dnext:f_decl option)):f_decl list =
     // turn "val f ... let f ..." into "let f..."
     match (d, dnext) with
     | (None, _) -> []
     | (Some d, None) -> [d]
-    | (Some d, Some dnext) when d.d_name = dnext.d_name -> []
+    | (Some d, Some dnext) when d.f_name = dnext.f_name -> []
     | (Some d, Some _) -> [d]
     in
-  let filter_decl (d:decl):bool =
-    List.forall (fun x -> x <> "private") d.d_qualifiers
+  let filter_decl (d:f_decl):bool =
+    List.forall (fun x -> x <> "private") d.f_qualifiers
     in
-  let abstract_decl (d:decl):decl =
-    if List.forall (fun x -> x <> "abstract") d.d_qualifiers then d else
-    {d with d_body = None}
+  let abstract_decl (d:f_decl):f_decl =
+    if List.forall (fun x -> x <> "abstract") d.f_qualifiers then d else
+    {d with f_body = None}
     in
   let ds_opt = List.map Some ds in
   let ds_prev = ds_opt @ [None] in
@@ -323,27 +328,27 @@ let filter_decls (ds:decl list):decl list =
   let ds = List.map abstract_decl ds in
   ds
 
-// Move a:Type _ from d_typ into d_binders
-let decl_lift_type_binders (d:decl):decl =
-  let rec f (d:decl):decl option =
-    match d.d_typ with
+// Move a:Type _ from f_typ into f_binders
+let decl_lift_type_binders (d:f_decl):f_decl =
+  let rec f (d:f_decl):f_decl option =
+    match d.f_typ with
     | EArrow (a, x, k, EApp (EAppUnivs (EId {name = Some ("Prims.Tot" | "Prims.GTot" | "Tot" | "GTot")}, _), [(_, t)]))
     | EArrow (a, x, k, EApp (EId {name = Some ("Prims.Tot" | "Prims.GTot" | "Tot" | "GTot")}, [(_, t)]))
     | EArrow (a, x, k, t) ->
         let (body, x) =
-          match d.d_body with
+          match d.f_body with
           | Some (EFun ([(_, x, _)], e)) -> (Some e, x)
           | Some (EFun ((_, x, _)::bs, e)) -> (Some (EFun (bs, e)), x)
           | _ -> (None, x)
           in
-        let d = {d with d_binders = d.d_binders @ [(a, x, Some k)]; d_typ = t; d_body = body} in
+        let d = {d with f_binders = d.f_binders @ [(a, x, Some k)]; f_typ = t; f_body = body} in
         f d
     | EType _ -> Some d
     | _ -> None
     in
   match f d with None -> d | Some d -> d
 
-let rec unsupported (e:exp):string option =
+let rec unsupported (e:f_exp):string option =
   match e with
   | EId x -> None
   | EInt i -> None
@@ -351,6 +356,10 @@ let rec unsupported (e:exp):string option =
   | EBool -> None
   | EProp -> None
   | EType u -> None
+  | EComp (EAppUnivs (EId {name = Some ("Prims.Pure" | "Prims.Ghost" | "Prims.Lemma")}, _), e1, _) when not keep_req_ens ->
+      unsupported e1
+  | EComp (EId {name = Some ("Prims.Pure" | "Prims.Ghost" | "Prims.Lemma")}, e1, _) when not keep_req_ens ->
+      unsupported e1
   | EComp (e1, e2, es) -> exps_unsupported (e1::e2::es)
   | EApp (e, aes) -> exps_unsupported (e::(List.map snd aes))
   | EAppUnivs (e, us) -> unsupported e
@@ -364,10 +373,10 @@ let rec unsupported (e:exp):string option =
   | ELet (b, e1, e2) -> exps_unsupported (e1::e2::(binder_exps b))
   | EFun (bs, e) -> exps_unsupported (e::(List.collect binder_exps bs))
   | EUnsupported s -> Some s
-and binder_exps (b:binder):exp list =
+and binder_exps (b:f_binder):f_exp list =
   let (_, _, e_opt) = b in
   list_opt e_opt (fun e -> [e])
-and exps_unsupported (es:exp list):string option =
+and exps_unsupported (es:f_exp list):string option =
   list_unsupported (List.map unsupported es)
 and list_unsupported (ss:string option list):string option =
   match ss with
@@ -375,19 +384,19 @@ and list_unsupported (ss:string option list):string option =
   | (Some s)::_ -> Some s
   | None::t -> list_unsupported t
 
-let decl_unsupported (d:decl):decl =
-  let u_binders = exps_unsupported (List.collect binder_exps d.d_binders) in
-  let u_typ = unsupported d.d_typ in
+let decl_unsupported (d:f_decl):f_decl =
+  let u_binders = exps_unsupported (List.collect binder_exps d.f_binders) in
+  let u_typ = unsupported d.f_typ in
   let body_opt =
-    match d.d_body with
+    match d.f_body with
     | None -> None
     | Some e -> match unsupported e with None -> Some e | Some _ -> None
     in
-  let d = {d with d_body = body_opt} in
+  let d = {d with f_body = body_opt} in
   let u = list_unsupported [u_binders; u_typ] in
   match u with
   | None -> d
-  | Some s -> {d with d_udecls = []; d_binders = []; d_typ = EUnsupported s; d_body = None}
+  | Some s -> {d with f_udecls = []; f_binders = []; f_typ = EUnsupported s; f_body = None}
 
 let rec index_to_var_id (xs:string list) (id:id):id =
   match id with
@@ -407,7 +416,7 @@ let rec index_to_var_univ (xs:string list) (u:univ):univ =
   | UPlus (u1, u2) -> UPlus (r u1, r u2)
   | UMax us -> UMax (List.map r us)
 
-let rec index_to_var_exp (xs:string list) (e:exp):exp =
+let rec index_to_var_exp (xs:string list) (e:f_exp):f_exp =
   let r = index_to_var_exp xs in
   match e with
   | EArrow (_, {name = None}, _, _)
@@ -435,7 +444,7 @@ let rec index_to_var_exp (xs:string list) (e:exp):exp =
       let (xs, bs) = index_to_var_binders xs bs in
       EFun (bs, index_to_var_exp xs e)
   | EUnsupported s -> e
-and index_to_var_binders (xs:string list) (bs:binder list):(string list * binder list) =
+and index_to_var_binders (xs:string list) (bs:f_binder list):(string list * f_binder list) =
   match bs with
   | [] -> (xs, bs)
   | (_, {name = None}, _)::_
@@ -446,22 +455,22 @@ and index_to_var_binders (xs:string list) (bs:binder list):(string list * binder
       let (xs, bs) = index_to_var_binders (x::xs) bs in
       (xs, (a, id, e_opt)::bs)
 
-let index_to_var_decl (d:decl):decl =
+let index_to_var_decl (d:f_decl):f_decl =
   let id_name (id:id):string =
     match id with
     | {name = None}
-    | {index = Some _} -> err ("index_to_var_decl: " + d.d_name)
+    | {index = Some _} -> err ("index_to_var_decl: " + d.f_name)
     | {name = Some x} -> x
     in
   try
-    let xs = List.rev (List.map id_name d.d_udecls) in
-    let (xs, bs) = index_to_var_binders xs d.d_binders in
-    let t = index_to_var_exp xs d.d_typ in
-    let body = Option.map (index_to_var_exp xs) d.d_body in
-    {d with d_binders = bs; d_typ = t; d_body = body}
+    let xs = List.rev (List.map id_name d.f_udecls) in
+    let (xs, bs) = index_to_var_binders xs d.f_binders in
+    let t = index_to_var_exp xs d.f_typ in
+    let body = Option.map (index_to_var_exp xs) d.f_body in
+    {d with f_binders = bs; f_typ = t; f_body = body}
   with
   | :? System.ArgumentException ->
-      {d with d_binders = []; d_typ = EUnsupported "bad variable index"; d_body = None}
+      {d with f_binders = []; f_typ = EUnsupported "bad variable index"; f_body = None}
 
 let rec universe0_univ_int (u:univ):bigint =
   let r = universe0_univ_int in
@@ -475,7 +484,7 @@ let rec universe0_univ_int (u:univ):bigint =
 let universe0_univ (u:univ):univ =
   UInt (universe0_univ_int u)
 
-let rec universe0_exp (e:exp):exp =
+let rec universe0_exp (e:f_exp):f_exp =
   let r = universe0_exp in
   match e with
   | EId {name = Some "Prims.bool"} -> EBool
@@ -492,50 +501,50 @@ let rec universe0_exp (e:exp):exp =
   | EPattern (pats, e) -> EPattern (List.map (List.map r) pats, r e)
   | ELet (b, e1, e2) -> ELet (universe0_binder b, r e1, r e2)
   | EFun (bs, e) -> EFun (List.map universe0_binder bs, r e)
-and universe0_binder (b:binder):binder =
+and universe0_binder (b:f_binder):f_binder =
   match b with
   | (a, x, e_opt) ->
       (a, x, Option.map universe0_exp e_opt)
 
-let universe0_decl (d:decl):decl =
+let universe0_decl (d:f_decl):f_decl =
   let (++) = Set.union in
-  let bs = List.map universe0_binder d.d_binders in
-  let body = Option.map universe0_exp d.d_body in
+  let bs = List.map universe0_binder d.f_binders in
+  let body = Option.map universe0_exp d.f_body in
   let t =
     // more sketchy Type(0) vs prop heuristics:
-    match (d.d_typ, body) with
-    | (EType (UInt i), None) when i.Equals(bigint.Zero) -> d.d_typ
+    match (d.f_typ, body) with
+    | (EType (UInt i), None) when i.Equals(bigint.Zero) -> d.f_typ
     | (EType (UInt i), Some e) when i.Equals(bigint.Zero) ->
       (
         match e with
-        | EApp (EId {name = Some "Prims.squash"}, _) -> universe0_exp d.d_typ
-        | EId _ | EApp _ | ERefine _ -> d.d_typ
-        | _ -> universe0_exp d.d_typ
+        | EApp (EId {name = Some "Prims.squash"}, _) -> universe0_exp d.f_typ
+        | EId _ | EApp _ | ERefine _ -> d.f_typ
+        | _ -> universe0_exp d.f_typ
       )
-    | _ -> universe0_exp d.d_typ
+    | _ -> universe0_exp d.f_typ
     in
-  {d with d_udecls = []; d_binders = bs; d_typ = t; d_body = body}
+  {d with f_udecls = []; f_binders = bs; f_typ = t; f_body = body}
 
-type env = Map<string, decl>
+type env = Map<string, f_decl>
 let reason = ref (None:string option)
 let set_reason (s:string):unit =
   match !reason with Some _ -> () | None -> reason := Some s
 
-let rec take_arrows (e:exp):(exp list * exp) =
+let rec take_arrows (e:f_exp):(f_exp list * f_exp) =
   match e with
   | EArrow (_, x, e1, e2) ->
       let (es, e) = take_arrows e2 in
       (e1::es, e)
   | _ -> ([], e)
 
-let rec is_vale_type (outer:bool) (leftmost:bool) (env:env) (e:exp):bool =
-  //printfn "is_vale_type? %s" (string_of_exp e);
+let rec is_vale_type (outer:bool) (leftmost:bool) (env:env) (e:f_exp):bool =
+  // printfn "// is_vale_type? %s" (string_of_exp e);
   //let r e = let b = is_vale_type false false env e in printfn "is_vale_type %A %s" b (string_of_exp e); b in
   let r = is_vale_type false false env in
   let may_be_refine e =
     match e with
     | ERefine ({name = Some x}, e1, e2) when outer ->
-        let dx = { d_name = x; d_qualifiers = []; d_category = "val"; d_udecls = []; d_binders = []; d_typ = e1; d_body = None} in
+        let dx = { f_name = x; f_qualifiers = []; f_category = "val"; f_udecls = []; f_binders = []; f_typ = e1; f_body = None} in
         let env = Map.add x dx env in
         //printfn "%A %A" (r e1) (is_vale_exp env e2);
         r e1 && is_vale_exp env e2
@@ -546,23 +555,26 @@ let rec is_vale_type (outer:bool) (leftmost:bool) (env:env) (e:exp):bool =
   | EBool -> true
   | EProp -> true
   | EComp (EId {name = Some ("Prims.Pure" | "Prims.Ghost" | "Prims.Lemma")}, e1, [er; EFun ([(_, {name = Some xe}, _)], ee)]) when outer ->
-      let dxe = { d_name = xe; d_qualifiers = []; d_category = "val"; d_udecls = []; d_binders = []; d_typ = e1; d_body = None} in
+      let dxe = { f_name = xe; f_qualifiers = []; f_category = "val"; f_udecls = []; f_binders = []; f_typ = e1; f_body = None} in
       let env2 = Map.add xe dxe env in
       //printfn "%A %A %A" (r e1) (is_vale_exp env er) (is_vale_exp env2 ee);
-      r e1 && is_vale_exp env er && is_vale_exp env2 ee
+      if keep_req_ens then
+        r e1 && is_vale_exp env er && is_vale_exp env2 ee
+      else
+        r e1
   | EComp (EId {name = Some ("Prims.Tot" | "Prims.GTot")}, e, [])
   | EApp (EId {name = Some ("Tot" | "GTot")}, [(_, e)]) ->
       may_be_refine e
   | EApp (e, aes) -> is_vale_type_id env e && List.forall r (List.map snd aes)
   | EArrow (_, {name = Some x}, ((EType (UInt i)) as t), e2) when leftmost && i.Equals(bigint.Zero) ->
-      let dx = { d_name = x; d_qualifiers = []; d_category = "type"; d_udecls = []; d_binders = []; d_typ = t; d_body = None} in
+      let dx = { f_name = x; f_qualifiers = []; f_category = "type"; f_udecls = []; f_binders = []; f_typ = t; f_body = None} in
       let env = Map.add x dx env in
       is_vale_type outer true env e2
   | EArrow (_, {name = Some x}, ((EType (UInt i)) as t), e2) when not leftmost && i.Equals(bigint.Zero) ->
       set_reason ("type parameters must be in outermost position: " + x); false
   | EArrow (a, {name = Some x}, e1, e2) ->
     (
-      let dx = { d_name = x; d_qualifiers = []; d_category = "val"; d_udecls = []; d_binders = []; d_typ = e1; d_body = None} in
+      let dx = { f_name = x; f_qualifiers = []; f_category = "val"; f_udecls = []; f_binders = []; f_typ = e1; f_body = None} in
       let env = Map.add x dx env in
       let b = may_be_refine e1 && is_vale_type outer false env e2 in
       match a with Explicit -> b | _ -> set_reason ("non-type parameters must be explicit, not inferred: " + x); false
@@ -570,18 +582,18 @@ let rec is_vale_type (outer:bool) (leftmost:bool) (env:env) (e:exp):bool =
   // TODO: more cases
   | EUnsupported s -> set_reason s; false
   | _ -> set_reason ("not vale type: " + string_of_exp e); false
-and is_vale_type_id (env:env) (e:exp):bool =
+and is_vale_type_id (env:env) (e:f_exp):bool =
   match e with
   | EId {name = Some "Prims.logical"} -> true
   | EId {name = Some x} ->
     (
       match Map.tryFind x env with
       // REVIEW: is any "type" ok?
-      | Some { d_category = "type" } -> true
+      | Some { f_category = "type" } -> true
       | _ -> set_reason x; false
     )
   | _ -> false
-and is_vale_exp (env:env) (e:exp):bool =
+and is_vale_exp (env:env) (e:f_exp):bool =
   //printfn "is_vale_exp? %s" (string_of_exp e);
   let r = is_vale_exp env in
   match e with
@@ -593,9 +605,9 @@ and is_vale_exp (env:env) (e:exp):bool =
       match get_vale_exp_id env e with
       | None -> false
       | Some d ->
-          let (ts, _) = take_arrows d.d_typ in
+          let (ts, _) = take_arrows d.f_typ in
           if List.length ts <> List.length aes then false else
-          let f (t:exp) (e:exp):bool =
+          let f (t:f_exp) (e:f_exp):bool =
             match t with
             | EType _ -> is_vale_type false false env e
             | _ -> is_vale_exp env e
@@ -605,23 +617,23 @@ and is_vale_exp (env:env) (e:exp):bool =
   // TODO: more cases
   | EUnsupported s -> set_reason s; false
   | _ -> set_reason ("not vale expression: " + string_of_exp e); false
-and get_vale_exp_id (env:env) (e:exp):decl option =
+and get_vale_exp_id (env:env) (e:f_exp):f_decl option =
   match e with
   | EId {name = Some x} ->
     (
       match Map.tryFind x env with
-      | Some ({ d_category = "val" } as d) -> Some d
+      | Some ({ f_category = "val" } as d) -> Some d
       | _ -> set_reason x; None
     )
   | _ -> None
 
-let as_int_constant (env:env) (e:exp):bigint option =
+let as_int_constant (env:env) (e:f_exp):bigint option =
   match e with
   | EInt i -> Some i
   | EId {name = Some x} when Map.containsKey x env ->
     (
       match Map.find x env with
-      | {d_category = "val"; d_udecls = []; d_binders = []; d_body = Some (EInt i)} -> Some i
+      | {f_category = "val"; f_udecls = []; f_binders = []; f_body = Some (EInt i)} -> Some i
       | _ -> None
     )
   | _ -> None
@@ -640,7 +652,7 @@ let range_intersect (r1:range) (r2:range):range =
 
 // Turn an expression about range_var into a range
 // Example: (5 <= range_var /\ range_var <= 10) becomes (Some 5, Some 10)
-let rec as_range_constant (local_env:Map<string, bigint>) (range_var:string) (e:exp):range option =
+let rec as_range_constant (local_env:Map<string, bigint>) (range_var:string) (e:f_exp):range option =
   let r = as_range_constant local_env range_var in
   let binary_op (flip:bool) (xop:string) (i:bigint):range option =
     match (xop, flip) with
@@ -654,7 +666,7 @@ let rec as_range_constant (local_env:Map<string, bigint>) (range_var:string) (e:
     | ("Prims.op_GreaterThan", true) -> Some (None, Some (i - bigint.One))
     | _ -> None
     in
-  let binary_op_exp (flip:bool) (xop:string) (e:exp):range option =
+  let binary_op_exp (flip:bool) (xop:string) (e:f_exp):range option =
     match e with
     | EInt i -> binary_op flip xop i
     | EId {name = Some x} when Map.containsKey x local_env ->
@@ -676,46 +688,49 @@ let rec as_range_constant (local_env:Map<string, bigint>) (range_var:string) (e:
       binary_op_exp true xop e
   | _ -> None
 
-let to_vale_decl ((env:env), (envs_ds_rev:(env * decl) list)) (d:decl):(env * (env * decl) list) =
+let to_vale_decl ((env:env), (envs_ds_rev:(env * f_decl) list)) (d:f_decl):(env * (env * f_decl) list) =
   let d = universe0_decl d in
-  let bs = d.d_binders in
+  let bs = d.f_binders in
   let bs_are_Type = List.forall (fun (_, _, e) -> match e with (Some (EType _)) -> true | _ -> false) bs in
-  //printfn "examining %s" d.d_name;
+  // printfn "// examining %s" d.f_name;
   reason := None;
   let typed_binders = List.forall (fun (_, _, t) -> Option.isSome t) in
-  let rec add_binders (bs:binder list) (e:exp):exp =
+  let rec add_binders (bs:f_binder list) (e:f_exp):f_exp =
     match bs with
     | [] -> e
     | (a, x, t_opt)::bs -> EArrow (a, x, Option.get t_opt, add_binders bs e)
     in
   let envs_ds =
-    match (bs, d.d_typ) with
+    let eInt = EId {name = Some "int"; index = None} in
+    let eIntRange = EId {name = Some "int_range"; index = None} in
+    match (bs, d.f_typ) with
     | (_, EType _) ->
+      (
         let body =
-          match (bs, d.d_body) with
+          match (bs, d.f_body) with
           // TODO: handle case with binders
           | ([], Some t) when is_vale_type false false env t -> Some t
           | _ -> None
           in
-        let int_refine:(range option * (Map<string, bigint> option * string * exp) option) option =
+        let int_refine:(range option * (Map<string, bigint> option * string * f_exp) option) option =
           // t           --> Some (Some range(t), None)
           // x:t{bounds} --> Some (Some range(t), Some (None, x, bounds))
-          if d.d_name = "Prims.int" then Some (Some (None, None), None) else
-          let int_type_to_range (e:exp):range option =
+          if d.f_name = "Prims.int" then Some (Some (None, None), None) else
+          let int_type_to_range (e:f_exp):range option =
             match e with
             | EId {name = Some "int"} -> Some (None, None)
-            | EApp (EId {name = Some "int"}, [(_, b1); (_, b2)]) ->
+            | EApp (EId {name = Some "int_range"}, [(_, b1); (_, b2)]) ->
                 let get_bound b = match b with | EInt i -> Some i | _ -> None in
                 Some (get_bound b1, get_bound b2)
             | _ -> None
             in
           let get_int_type (x:string):range option =
             match Map.tryFind x env with
-            | Some {d_category = "type"; d_udecls = []; d_binders = []; d_body = Some e} ->
+            | Some {f_category = "type"; f_udecls = []; f_binders = []; f_body = Some e} ->
                 int_type_to_range e
             | _ -> None
             in
-          match d.d_body with
+          match d.f_body with
           | Some (EId {name = Some xt}) -> Some (get_int_type xt, None)
           | Some (EApp (EId {name = Some xt}, args)) ->
               let args = List.map snd args in
@@ -723,7 +738,7 @@ let to_vale_decl ((env:env), (envs_ds_rev:(env * decl) list)) (d:decl):(env * (e
               if List.forall Option.isSome args then
                 let args = List.map Option.get args in
                 match Map.tryFind xt env with
-                | Some {d_category = "int_type_generator"; d_binders = bs; d_body = Some (ERefine ({name = Some xr}, et, bounds))}
+                | Some {f_category = "int_type_generator"; f_binders = bs; f_body = Some (ERefine ({name = Some xr}, et, bounds))}
                     when List.length bs = List.length args ->
                     let add_x_i env x i = Map.add x i env in
                     let xs = List.map (fun (_, (x:id), _) -> Option.get x.name) bs in
@@ -736,9 +751,7 @@ let to_vale_decl ((env:env), (envs_ds_rev:(env * decl) list)) (d:decl):(env * (e
               Some (get_int_type xt, Some (None, xr, bounds))
           | _ -> None
           in
-        let range_to_int_type (r:range):exp =
-          let eInt = EId {name = Some "int"; index = None} in
-          let eIntRange = EId {name = Some "int_range"; index = None} in
+        let range_to_int_type (r:range):f_exp =
           let eNone = EId {name = Some "_"; index = None} in
           match r with
           | (None, None) -> eInt
@@ -749,22 +762,22 @@ let to_vale_decl ((env:env), (envs_ds_rev:(env * decl) list)) (d:decl):(env * (e
         let int_refine = match int_refine with Some (Some r, z) -> Some (r, z) | _ -> None in
         match (bs, bs_are_Type, int_refine) with
         | (_, true, None) ->
-            [(env, {d with d_category = "type"; d_body = body})]
+            [(env, {d with f_category = "type"; f_body = body})]
         | (_, false, None) ->
-            [(env, {d with d_category = "unsupported"; d_typ = EUnsupported "dependent type"})]
+            [(env, {d with f_category = "unsupported"; f_typ = EUnsupported "dependent type"})]
         | ([], _, Some (r, None)) ->
-            [(env, {d with d_category = "type"; d_body = Some (range_to_int_type r)})]
+            [(env, {d with f_category = "type"; f_body = Some (range_to_int_type r)})]
         | ([], _, Some (r, Some (local_env_bounds_opt, xr, bounds))) ->
           (
             let local_env_bounds = Option.defaultValue Map.empty local_env_bounds_opt in
             match as_range_constant local_env_bounds xr bounds with
             | None ->
-                [(env, {d with d_category = "unsupported"; d_typ = EUnsupported "unsupported integer bounds"})]
+                [(env, {d with f_category = "unsupported"; f_typ = EUnsupported "unsupported integer bounds"})]
             | Some r_bounds ->
-                [(env, {d with d_category = "type"; d_body = Some (range_to_int_type (range_intersect r r_bounds))})]
+                [(env, {d with f_category = "type"; f_body = Some (range_to_int_type (range_intersect r r_bounds))})]
           )
         | (_, false, Some (r, Some (None, xr, bounds))) ->
-            let rec resolve_bounds (e:exp):exp =
+            let rec resolve_bounds (e:f_exp):f_exp =
               match (as_int_constant env e, e) with
               | (Some i, _) -> EInt i
               | (_, EApp (e0, es)) -> EApp (e0, List.map (fun (a, e) -> (a, resolve_bounds e)) es)
@@ -772,21 +785,22 @@ let to_vale_decl ((env:env), (envs_ds_rev:(env * decl) list)) (d:decl):(env * (e
               in
             let bounds = resolve_bounds bounds in
             let body = ERefine ({name = Some xr; index = None}, range_to_int_type r, bounds) in
-            [(env, {d with d_category = "int_type_generator"; d_body = Some body})]
+            [(env, {d with f_category = "int_type_generator"; f_body = Some body})]
         | _ ->
-            [(env, {d with d_category = "unsupported"; d_typ = EUnsupported "unsupported"})]
-    | (bs, _) when typed_binders bs && is_vale_type true true env (add_binders bs d.d_typ) ->
-        let body =
-          match (bs, Option.bind (as_int_constant env) d.d_body) with
-          | ([], Some i) -> Some (EInt i)
-          | _ -> None
+            [(env, {d with f_category = "unsupported"; f_typ = EUnsupported "unsupported"})]
+      )
+    | (bs, _) when typed_binders bs && is_vale_type true true env (add_binders bs d.f_typ) ->
+        let (body, t) =
+          match (bs, Option.bind (as_int_constant env) d.f_body) with
+          | ([], Some i) -> (Some (EInt i), EApp (eIntRange, [(Explicit, EInt i); (Explicit, EInt i)]))
+          | _ -> (None, d.f_typ)
           in
-        [(env, {d with d_category = "val"; d_body = body})]
+        [(env, {d with f_category = "val"; f_body = body; f_typ = t})]
     | _ ->
-        let t = match !reason with None -> d.d_typ | Some s -> EUnsupported s in
-        [(env, {d with d_category = "unsupported"; d_typ = t})]
+        let t = match !reason with None -> d.f_typ | Some s -> EUnsupported s in
+        [(env, {d with f_category = "unsupported"; f_typ = t})]
     in
-  let env = List.fold (fun env (_, d) -> Map.add d.d_name d env) env envs_ds in
+  let env = List.fold (fun env (_, d) -> Map.add d.f_name d env) env envs_ds in
   let envs_ds_rev = envs_ds @ envs_ds_rev in
   (env, envs_ds_rev)
 
@@ -796,81 +810,110 @@ let rec trees_of_comma_list (es:string_tree list):string_tree list =
   | [e] -> [e]
   | e::es -> (st_list [e; st_leaf ","])::(trees_of_comma_list es)
 
-let rec tree_of_vale_name (x:string):string_tree =
-  let r = tree_of_vale_name in
+let rec string_of_vale_name (x:string):string =
+  let r = string_of_vale_name in
   match x with
 //  | ("Prop_s.prop0" | "Prims.prop" | "Prims.logical") -> st_leaf "prop"
   | _ when x.EndsWith(".decreases") -> r (x.Replace(".decreases", "._decreases"))
   | _ when x.EndsWith(".modifies") -> r (x.Replace(".modifies", "._modifies"))
   | _ ->
       let x = if x.StartsWith("'") then "_" + x else x in
-      st_leaf (x.Replace("#", "_"))
+      x.Replace("#", "_")
 
-let tree_of_vale_id (id:id):string_tree =
+let vale_string_of_id (id:id):string =
   match id with
-  | {name = Some x} -> tree_of_vale_name x
-  | _ -> err ("internal error: tree_of_vale_id: " + string_of_id id)
+  | {name = Some x} -> string_of_vale_name x
+  | _ -> err ("internal error: vale_string_of_id: " + string_of_id id)
 
-let tree_of_vale_kind (e:exp):string_tree =
+let vale_kind_of_exp (e:f_exp):v_kind =
   match e with
-  | EType (UInt i) -> st_leaf ("Type(" + i.ToString() + ")")
-  | _ -> err ("internal error: tree_of_vale_kind: " + string_of_exp e)
+  | EType (UInt i) -> KType i
+  | _ -> err ("internal error: vale_kind_of_f_exp: " + string_of_exp e)
 
-let rec tree_of_vale_type (e:exp):string_tree =
-  let r = tree_of_vale_type in
+let rec vale_type_of_exp (e:f_exp):v_type =
+  let r = vale_type_of_exp in
   match e with
-  | EId id -> tree_of_vale_id id
-  | EInt i -> st_leaf (i.ToString())
-  | EBool -> st_leaf "bool"
-  | EProp -> st_leaf "prop"
-  | EComp (EId {name = Some ("Prims.Tot" | "Prims.GTot")}, e, [])
+  | EId id -> TName (vale_string_of_id id)
+  | EInt i -> TInt i
+  | EBool -> TName "bool"
+  | EProp -> TName "prop"
+  | EComp (EId {name = Some ("Prims.Tot" | "Prims.GTot")}, e, []) -> r e
   | EApp (EId {name = Some ("Tot" | "GTot")}, [(_, e)]) -> r e
-  | EApp (e, aes) ->
+  | EApp (EId {name = Some x}, aes) ->
       // TODO: tuples are special case
-      st_paren [r e; st_paren (trees_of_comma_list (List.map (snd >> r) aes))]
+      TApply (string_of_vale_name x, List.map (snd >> r) aes)
   | EArrow _ ->
       let (es, e) = take_arrows e in
-      st_paren [st_leaf "fun"; st_paren (trees_of_comma_list (List.map r es)); st_leaf "->"; r e]
-  | _ -> err ("internal error: tree_of_vale_type: " + string_of_exp e)
+      TFun (List.map r es, r e)
+  | _ -> err ("internal error: vale_type_of_exp: " + string_of_exp e)
 
-let tree_of_vale_type_kind (e:exp):string_tree =
+let rec vale_exp_of_exp (env:env) (e:f_exp):v_exp =
+  let r = vale_exp_of_exp env in
   match e with
-  | EType _ -> tree_of_vale_kind e
-  | _ -> tree_of_vale_type e
-
-let rec tree_of_vale_exp (env:env) (e:exp):string_tree =
-  let r = tree_of_vale_exp env in
-  match e with
-  | EId x -> tree_of_vale_id x
-  | EInt i -> st_leaf (i.ToString())
-  | EUnitValue -> st_leaf "tuple()"
-  | EApp (e, aes) ->
+  | EId x -> VId (vale_string_of_id x)
+  | EInt i -> VInt i
+  | EUnitValue -> VApp ("tuple", None, [])
+  | EApp (EId x as e, aes) ->
       let ts =
         match get_vale_exp_id env e with
-        | None -> List.map (fun _ -> e) aes // not a top-level decl; no type arguments allowed
-        | Some d -> fst (take_arrows d.d_typ)
+        | None -> List.map (fun _ -> e) aes // not a top-level f_decl; no type arguments allowed
+        | Some d -> fst (take_arrows d.f_typ)
         in
-      let f (t:exp) (e:exp):string_tree =
-        match t with
-        | EType _ -> tree_of_vale_type e
-        | _ -> tree_of_vale_exp env e
-        in
-      let ss = List.map2 f ts (List.map snd aes) in
-      st_paren [r e; st_paren (trees_of_comma_list ss)]
+      let es_ts = List.map2 (fun t (_, e) -> (t, e)) ts aes in
+      let (ts, es) = List.partition (fun (t, _) -> match t with EType _ -> true | _ -> false) es_ts in
+      let ts = List.map (snd >> vale_type_of_exp) ts in
+      let es = List.map (snd >> (vale_exp_of_exp env)) es in
+      VApp (vale_string_of_id x, (match ts with [] -> None | _ -> Some ts), es)
   | ELet ((_, x, Some t), e1, e2) ->
-      st_paren [st_list [st_leaf "let"; tree_of_vale_id x; st_leaf ":"; tree_of_vale_type t; st_leaf ":="; r e1; st_leaf "in"]; r e2]
-  | _ -> err ("internal error: tree_of_vale_exp: " + string_of_exp e)
+      VLet (vale_string_of_id x, vale_type_of_exp t, r e1, r e2)
+  | _ -> err ("internal error: vale_exp_of_exp: " + string_of_exp e)
+
+let tree_of_vale_name (x:string):string_tree =
+  st_leaf (string_of_vale_name x)
+
+let tree_of_vale_id (id:id):string_tree =
+  st_leaf (vale_string_of_id id)
+
+let tree_of_vale_kind ((KType i):v_kind):string_tree =
+  st_leaf ("Type(" + i.ToString() + ")")
+
+let rec tree_of_vale_type (t:v_type):string_tree =
+  let r = tree_of_vale_type in
+  match t with
+  | TName id -> st_leaf id
+  | TInt i -> st_leaf (i.ToString())
+  | TApply (x, ts) ->
+      st_paren [st_leaf x; st_paren (trees_of_comma_list (List.map r ts))]
+  | TFun (ts, t) ->
+      st_paren [st_leaf "fun"; st_paren (trees_of_comma_list (List.map r ts)); st_leaf "->"; r t]
+
+let tree_of_vale_type_kind (e:f_exp):string_tree =
+  match e with
+  | EType _ -> tree_of_vale_kind (vale_kind_of_exp e)
+  | _ -> tree_of_vale_type (vale_type_of_exp e)
+
+let rec tree_of_vale_exp (e:v_exp):string_tree =
+  let r = tree_of_vale_exp in
+  match e with
+  | VId x -> st_leaf x
+  | VInt i -> st_leaf (i.ToString())
+  | VApp (x, None, es) ->
+      st_paren [st_leaf x; st_paren (trees_of_comma_list (List.map r es))]
+  | VApp (x, Some ts, es) ->
+      st_paren [st_leaf x; st_hash_bracket (trees_of_comma_list (List.map tree_of_vale_type ts)); st_paren (trees_of_comma_list (List.map r es))]
+  | VLet (x, t, e1, e2) ->
+      st_paren [st_list [st_leaf "let"; st_leaf x; st_leaf ":"; tree_of_vale_type t; st_leaf ":="; r e1; st_leaf "in"]; r e2]
 
 // returns parameters, requires, ensures, return type
-let rec take_params (e:exp):(binder list * exp list * (id * exp) option * exp) =
-  let may_be_refine_req (x:id) (e:exp):(exp list * exp) =
+let rec take_params (e:f_exp):(f_binder list * f_exp list * (id * f_exp) option * f_exp) =
+  let may_be_refine_req (x:id) (e:f_exp):(f_exp list * f_exp) =
     match e with
     | ERefine (x1, e1, e2) ->
         let req = ELet ((Explicit, x1, Some e1), EId x, e2) in
         ([req], e1)
     | _ -> ([], e)
     in
-  let may_be_refine_ens (e:exp):((id * exp) option * exp) =
+  let may_be_refine_ens (e:f_exp):((id * f_exp) option * f_exp) =
     match e with
     | ERefine (x1, e1, e2) -> (Some (x1, e2), e1)
     | _ -> (None, e)
@@ -882,36 +925,39 @@ let rec take_params (e:exp):(binder list * exp list * (id * exp) option * exp) =
       let (bs, reqs, enss, e) = take_params e2 in
       (b::bs, req @ reqs, enss, e)
   | EComp (EId {name = Some ("Prims.Pure" | "Prims.Ghost" | "Prims.Lemma")}, e1, [req; EFun ([(_, xens, _)], ens)]) ->
-      ([], [req], Some (xens, ens), e1)
+      if keep_req_ens then
+        ([], [req], Some (xens, ens), e1)
+      else
+        ([], [], None, e1)
   | EComp (EId {name = Some ("Prims.Tot" | "Prims.GTot")}, e, [])
   | EApp (EId {name = Some ("Tot" | "GTot")}, [(_, e)])
   | e ->
       let (ens, e) = may_be_refine_ens e in
       ([], [], ens, e)
 
-let tree_of_vale_decl (env:env) (d:decl):string_tree =
-  match d.d_category with
+let tree_of_vale_decl (env:env) (d:f_decl):string_tree =
+  match d.f_category with
   | "type" ->
     (
       let ps =
-        match d.d_binders with
+        match d.f_binders with
         | [] -> []
         | bs ->
-            let f (_, x, k) = st_list [tree_of_vale_id x; st_leaf ":"; tree_of_vale_kind (Option.get k)] in
+            let f (_, x, k) = st_list [tree_of_vale_id x; st_leaf ":"; tree_of_vale_kind (vale_kind_of_exp (Option.get k))] in
             [st_paren (trees_of_comma_list (List.map f bs))]
         in
-      let typing = [st_leaf ":"; tree_of_vale_kind d.d_typ] in
+      let typing = [st_leaf ":"; tree_of_vale_kind (vale_kind_of_exp d.f_typ)] in
       let body =
-        match d.d_body with
+        match d.f_body with
         | None -> [st_leaf "extern"; st_leaf ";"]
-        | Some t -> [st_leaf ":="; tree_of_vale_type t; st_leaf ";"]
+        | Some t -> [st_leaf ":="; tree_of_vale_type (vale_type_of_exp t); st_leaf ";"]
         in
-      st_list ([st_leaf "type"; tree_of_vale_name d.d_name] @ ps @ typing @ body)
+      st_list ([st_leaf "type"; tree_of_vale_name d.f_name] @ ps @ typing @ body)
     )
   | "val" ->
     (
-      let (bs, reqs, enss, t) = take_params d.d_typ in
-      let bs = d.d_binders @ bs in
+      let (bs, reqs, enss, t) = take_params d.f_typ in
+      let bs = d.f_binders @ bs in
       let (prefix, ps) =
         match bs with
         | [] -> ("const", [])
@@ -924,18 +970,18 @@ let tree_of_vale_decl (env:env) (d:decl):string_tree =
             let tparams = match bst with [] -> [] | _ -> [make_st_list "#[" "]" (trees_of_comma_list (List.map f bst))] in
             ("function", tparams @ [st_paren (trees_of_comma_list (List.map f bsv))])
         in
-      let tree_req = List.map (fun e -> st_list [st_leaf "requires"; tree_of_vale_exp env e; st_leaf ";"]) reqs in
-      let tree_t = tree_of_vale_type t in
+      let tree_req = List.map (fun e -> st_list [st_leaf "requires"; tree_of_vale_exp (vale_exp_of_exp env e); st_leaf ";"]) reqs in
+      let tree_t = tree_of_vale_type (vale_type_of_exp t) in
       let (tree_t, tree_ens) =
         match enss with
         | None -> (tree_t, [])
         | Some (x, e) ->
-            (st_paren [tree_of_vale_id x; st_leaf ":"; tree_t], [st_list [st_leaf "ensures"; tree_of_vale_exp env e; st_leaf ";"]])
+            (st_paren [tree_of_vale_id x; st_leaf ":"; tree_t], [st_list [st_leaf "ensures"; tree_of_vale_exp (vale_exp_of_exp env e); st_leaf ";"]])
         in
       let typing = [st_leaf ":"; tree_t] @ tree_req @ tree_ens @ [st_leaf "extern"; st_leaf ";"] in
-      st_list ([st_leaf prefix; tree_of_vale_name d.d_name] @ ps @ typing)
+      st_list ([st_leaf prefix; tree_of_vale_name d.f_name] @ ps @ typing)
     )
-  | _ -> err ("internal error: tree_of_vale_decl: " + d.d_category)
+  | _ -> err ("internal error: tree_of_vale_decl: " + d.f_category)
 
 let main (argv:string array) =
   let in_files_rev = ref ([]:string list) in
@@ -1014,7 +1060,7 @@ let main (argv:string array) =
       List.map (String.concat "\n") all_blocks
       in
     let blocks = List.collect read_file in_files in
-    let parse_block (s:string):decl list =
+    let parse_block (s:string):f_decl list =
       //printfn "%s" s;
       let bytes = System.Text.Encoding.UTF8.GetBytes(s) in
       let lexbuf = LexBuffer<byte>.FromBytes bytes in
@@ -1027,7 +1073,7 @@ let main (argv:string array) =
       let ds = List.map parse_decl res in
       let ds =
         match ds with
-        | d::_ when List.exists (fun s -> s = "abstract") d.d_qualifiers -> [d]
+        | d::_ when List.exists (fun s -> s = "abstract") d.f_qualifiers -> [d]
         | _ -> ds
         in
       ds
@@ -1042,14 +1088,14 @@ let main (argv:string array) =
     let duplicates = ref (Set.empty : Set<string>) in
     List.iter
       (fun (env, d) ->
-        if not (Set.contains d.d_name (!duplicates)) then
+        if not (Set.contains d.f_name (!duplicates)) then
          (
           // REVIEW: why are there duplicates?
-          duplicates := Set.add d.d_name (!duplicates);
-          match (d.d_category, d.d_typ) with
-          | (_, EUnsupported s) -> printfn "unsupported: %s //(reason: %s)" d.d_name s; printfn ""
-          | ("unsupported", _) -> printfn "unsupported: %s" d.d_name; printfn ""
-          | ("int_type_generator", _) -> printfn "unsupported (int type generator): %s" d.d_name; printfn ""
+          duplicates := Set.add d.f_name (!duplicates);
+          match (d.f_category, d.f_typ) with
+          | (_, EUnsupported s) -> printfn "unsupported: %s //(reason: %s)" d.f_name s; printfn ""
+          | ("unsupported", _) -> printfn "unsupported: %s" d.f_name; printfn ""
+          | ("int_type_generator", _) -> printfn "unsupported (int type generator): %s" d.f_name; printfn ""
           | _ -> print_tree "" (tree_of_vale_decl env d); printfn ""
          )
       )
