tools/Vale/test/FTypeFStar.fst
@@ -8,3 +8,10 @@ let id x = x
 //type list (a:Type0) : Type0 = | Nil : list a | Cons : a -> list a -> list a
 let nil = Nil
 let cons = Cons
+
+assume val xeq2 (#a:Type) (x:a) (y:a) : prop
+assume val ff1 (z:int) : Lemma (xeq2 10 20 /\ (match z with 3 -> True | _ -> False))
+assume val ff2 (z:int) : Pure int (requires True) (ensures fun _ -> xeq2 10 20 /\ (match z with 3 -> True | _ -> False))
+
+let natN (n:nat) = x:nat{x < n}
+let nat8 = natN 256
