src/arch/Types_i.fsti
@@ -5,5 +5,15 @@ open Words_s
 open Words.Four_s
 open Words.Two_s
 
+unfold let add_wrap64 (x:nat64) (y:nat64) : nat64 = add_wrap x y
+
+// abstract bitwise operations on integers:
+unfold let iand64 (a:nat64) (b:nat64) : nat64 = iand a b
+unfold let ixor64 (a:nat64) (b:nat64) : nat64 = ixor a b
+unfold let ior64 (a:nat64) (b:nat64) : nat64 = ior a b
+unfold let inot64 (a:nat64) : nat64 = inot a
+unfold let ishl64 (a:nat64) (s:int) : nat64 = ishl a s
+unfold let ishr64 (a:nat64) (s:int) : nat64 = ishr a s
+
 let lo64 (q:quad32) : nat64 = two_to_nat 32 (two_select (four_to_two_two q) 0)
 let hi64 (q:quad32) : nat64 = two_to_nat 32 (two_select (four_to_two_two q) 1)
